Add beginnings of the CEK machine

src/Eval.v
@@ -22,8 +22,10 @@ Inductive Eval : ∀ {τ}, Exp [] τ → Exp [] τ → Prop :=
     Eval e2 v → Eval (Seq e1 e2) v
   | EvNil τ :
     Eval (@Nil _ τ) Nil
-  | EvCons τ (x : Exp [] τ) (xs : Exp [] (TyList τ)) :
-    Eval (Cons x xs) (Cons x xs)
+  | EvCons τ (x : Exp [] τ) x' (xs : Exp [] (TyList τ)) xs' :
+    Eval x x' →
+    Eval xs xs' →
+    Eval (Cons x xs) (Cons x' xs')
   | EvLet τ ty (x : Exp [] ty) w (body : Exp [ty] τ) v :
     Eval x w →
     Eval (STmExp {| w |} body) v →
@@ -42,6 +44,9 @@ Theorem soundness τ (e : Exp [] τ) v :
 Proof.
   intros.
   induction H; simpl; auto.
+  - extensionality E.
+    destruct E.
+    now rewrite IHEval1, IHEval2.
   - extensionality E.
     destruct E.
     rewrite IHEval1.
