src/Exp.v
@@ -19,7 +19,7 @@ Inductive Var : Env → Ty → Type :=
 Derive Signature NoConfusion for Var.
 
 Inductive Exp Γ : Ty → Type :=
-  | Constant {τ}  : Literal τ → Exp Γ τ
+  | Constant {ty} : Literal ty → Exp Γ (TyPrim ty)
   | Seq {τ τ'}    : Exp Γ τ' → Exp Γ τ → Exp Γ τ
   | Nil {τ}       : Exp Γ (TyList τ)
   | Cons {τ}      : Exp Γ τ → Exp Γ (TyList τ) → Exp Γ (TyList τ)
@@ -37,7 +37,7 @@ End Exp.
 Arguments ZV {_ _}.
 Arguments SV {_ _ _} _.
 
-Arguments Constant {Γ τ} _.
+Arguments Constant {Γ ty} _.
 Arguments Seq {Γ τ τ'} _ _.
 Arguments Nil {Γ τ}.
 Arguments Cons {Γ τ} _ _.
