src/CEK.v
@@ -1,0 +1,134 @@
+Require Export
+  Ty
+  Exp
+  Sub
+  Sem
+  Eval.
+
+From Equations Require Import Equations.
+Set Equations With UIP.
+
+Generalizable All Variables.
+
+Import ListNotations.
+
+Section CEK.
+
+Inductive Value : Ty → Type :=
+  | VLit {ty} : Literal ty → Value (TyPrim ty)
+  | VNil {τ} : Value (TyList τ)
+  | VCons {τ} : Value τ → Value (TyList τ) → Value (TyList τ)
+  | VClosure {dom cod} : Closure (dom ⟶ cod) → Value (dom ⟶ cod)
+
+with Closure : Ty → Type :=
+  | Closed {Γ dom cod} : Exp (dom :: Γ) cod → Env Γ → Closure (dom ⟶ cod)
+
+with Env : Env → Type :=
+  | Empty : Env []
+  | Val {Γ τ} : Value τ → Env Γ → Env (τ :: Γ).
+
+Derive Signature NoConfusion Subterm for Value.
+Derive Signature NoConfusion Subterm for Closure.
+Derive Signature NoConfusion for Env.
+
+Equations get `(se : Env Γ) `(v : Var Γ τ) : Value τ :=
+  get (Val x _)   ZV    := x;
+  get (Val _ xs) (SV v) := get xs v.
+
+Inductive Kont : Ty → Ty → Type :=
+  | Mt {u} : Kont u u
+  | Ar {Γ u v w} : Exp Γ u → Env Γ → Kont v w → Kont (u ⟶ v) w
+  | Fn {a b c} : Closure (a ⟶ b) → Kont b c → Kont a c.
+
+Derive Signature NoConfusion for Kont.
+
+Record Σ := MkΣ {
+  Γ   : Exp.Env;
+  τ   : Ty;
+  exp : Exp Γ τ;
+  env : Env Γ;
+  r   : Ty;
+  knt : Kont τ r
+}.
+
+Arguments MkΣ {Γ τ} _ _ {r} _.
+
+Definition inject {τ : Ty} (e : Exp [] τ) : Σ := MkΣ e Empty Mt.
+
+Equations step (gas : nat) {Γ : Exp.Env} {τ : Ty} (e : Exp Γ τ) (ρ : Env Γ)
+          {r : Ty} `(κ : Kont τ r) : Σ :=
+  step 0 _ _ _ := MkΣ e ρ κ;
+
+  (* A constant is passed as a literal *)
+  step (S g) (Constant x) _ (Fn (Closed b ρ') κ) :=
+    step g b (Val (VLit x) ρ') κ;
+
+  (* A sequence just evaluates the second, for now *)
+  step (S g) (Seq e1 e2) ρ κ :=
+    step g e2 ρ κ;
+
+  (* Nil is just a special constant *)
+  step (S g) Nil _ (Fn (Closed b ρ') κ) :=
+    step g b (Val VNil ρ') κ;
+  (* Cons walk down the list evaluating all of the elements *)
+  step (S g) (Cons x xs) ρ κ :=
+    step g x ρ (Fn (Closed (Cons (VAR ZV) (wk xs)) ρ) κ);
+
+  (* Let is a simple desugaring *)
+  step (S g) (Let x body) ρ κ :=
+    step g (APP (LAM body) x) ρ κ;
+
+  (* A variable might lookup a lambda, in which case continue evaluating down
+     that vein; otherwise, if no continuation, this is as far as we can go. *)
+  step (S g) (VAR v) ρ κ with get ρ v := {
+    | VClosure (Closed e ρ') => step g (LAM e) ρ' κ
+    | x with κ := {
+        | Fn (Closed b ρ') κ' => step g b (Val x ρ') κ'
+        | Mt => step g (VAR v) ρ Mt
+      }
+  };
+
+  (* Lambda evaluates its argument, with the lambda as the cont *)
+  step (S g) (LAM e) ρ (Ar a ρ' κ) :=
+    step g a ρ' (Fn (Closed e ρ) κ);
+  (* If a lambda is being passed, call the continuation with it *)
+  step (S g) (LAM e) ρ (Fn (Closed b ρ') κ) :=
+    step g b (Val (VClosure (Closed e ρ)) ρ') κ;
+
+  (* Application evaluates the lambda and then the argument *)
+  step (S g) (APP e1 e2) ρ κ :=
+    step g e1 ρ (Ar e2 ρ κ);
+
+  (* Otherwise, there is nothing more than can be done *)
+  step _ s ρ Mt := MkΣ s ρ Mt.
+
+Definition run (gas : nat) {τ : Ty} (e : Exp [] τ) : Σ :=
+  step gas e Empty Mt.
+
+Theorem cek_sound τ (e : Exp [] τ) v :
+  Eval e v → ∃ gas, run gas e = MkΣ v Empty Mt.
+Proof.
+  unfold run, Basics.compose, inject.
+  intros.
+  induction H; simpl; intros; auto.
+  - exists 1%nat; simpl.
+    now rewrite step_equation_2.
+  - destruct IHEval as [gas' IHEval'].
+    now exists (S gas').
+  - exists 1%nat; simpl.
+    now rewrite step_equation_5.
+  - destruct IHEval1 as [gas1 IHEval1'].
+    destruct IHEval2 as [gas2 IHEval2'].
+    exists (S (S (S (gas1 + gas2)))).
+    rewrite step_equation_7.
+    admit.
+  - destruct IHEval1 as [gas1 IHEval1].
+    destruct IHEval2 as [gas2 IHEval2].
+    exists (S (S (S (gas1 + gas2)))).
+    rewrite step_equation_8.
+    rewrite step_equation_13.
+    rewrite step_equation_11.
+    admit.
+  - admit.
+  - admit.
+Abort.
